cogent/examples/wa_connect/Generated_CorresProof.thy
@@ -76,6 +76,14 @@ ML \<open>
 fun typing_tree_of "wordarray_get_u32" = wordarray_get_u32_typing_tree
   | typing_tree_of "wordarray_length_u32" = wordarray_length_u32_typing_tree
   | typing_tree_of "wordarray_put2_u32" = wordarray_put2_u32_typing_tree
+  | typing_tree_of "dec" = dec_typing_tree
+  | typing_tree_of "dec_arr" = dec_arr_typing_tree
+  | typing_tree_of "inc" = inc_typing_tree
+  | typing_tree_of "inc_arr" = inc_arr_typing_tree
+  | typing_tree_of "mul" = mul_typing_tree
+  | typing_tree_of "mul_arr" = mul_arr_typing_tree
+  | typing_tree_of "sum" = sum_typing_tree
+  | typing_tree_of "sum_arr" = sum_arr_typing_tree
   | typing_tree_of f = error ("No typing tree for " ^ quote f)
 \<close>
 ML \<open>
@@ -140,7 +148,15 @@ val Cogent_main_tree =
 val entry_func_names = [
       "wordarray_length_u32",
       "wordarray_get_u32",
-      "wordarray_put2_u32"
+      "wordarray_put2_u32",
+      "inc",
+      "dec",
+      "inc_arr",
+      "dec_arr",
+      "sum",
+      "mul",
+      "sum_arr",
+      "mul_arr"
 ]
 val entry_funcs = Symtab.dest Cogent_main_tree
       |> filter (fn (n, _) => member (op =) entry_func_names n) |> Symtab.make
